Fp/Basic.lean
@@ -304,11 +304,11 @@ def equal_denotation (a b : EFixedPoint w e) : Bool :=
 
 @[simp]
 def isNaN (a : EFixedPoint w e) : Bool :=
-  a.state == .NaN
+  a.state = .NaN
 
 @[simp]
 def isZero (a : EFixedPoint w e) : Bool :=
-  a.state == .Number && a.num.val == 0
+  a.state = .Number && a.num.val == 0
 
 end EFixedPoint
 
