Fp/Multiplication.lean
@@ -27,7 +27,7 @@ def e_mul (a : EFixedPoint v e) (b : EFixedPoint w f) : EFixedPoint (v+w) (e+f) 
       num := f_mul a.num b.num
     }
 
-def mul
+def mulfixed
   (he : 0 < e) (a b : PackedFloat e s) (m : RoundingMode) : PackedFloat e s :=
   round _ _ m (e_mul (a.toEFixed he) (b.toEFixed he))
 
@@ -43,12 +43,45 @@ theorem e_mul_comm (a b : EFixedPoint 34 16)
   cases ha2 : a.state <;> cases hb2 : b.state <;>
     simp_all [Bool.xor_comm, f_mul_comm]
 
-theorem mul_comm_brute (a b : EFixedPoint 4 2)
-  : (e_mul a b) = (e_mul b a) := by
-  apply EFixedPoint.inj
-  simp [e_mul, f_mul]
-  bv_decide +acNf
+theorem mulfixed_comm (a b : PackedFloat 5 2) (m : RoundingMode)
+  : (mulfixed (by omega) a b m) = (mulfixed (by omega) b a m) := by
+  simp [mulfixed, e_mul_comm]
+
+-- A bit-blastable version of multiplication, unrelated to fixed-point numbers
+def mul
+  (a b : PackedFloat e s) (m : RoundingMode) : PackedFloat e s :=
+  if a.isNaN || b.isNaN ||
+    (a.isInfinite && b.isZero) ||
+    (b.isInfinite && a.isZero) then PackedFloat.getNaN _ _
+  else if a.isInfinite || b.isInfinite then
+    PackedFloat.getInfinity _ _ (a.sign ^^ b.sign)
+  else
+    let sa := BitVec.cons (a.ex != 0) a.sig
+    let sb := BitVec.cons (b.ex != 0) b.sig
+    let shift : BitVec (e+1) :=
+      (if a.ex == 0 then 0 else a.ex - 1).setWidth _ +
+      (if b.ex == 0 then 0 else b.ex - 1).setWidth _
+    let prod := sa.setWidth (2*(s+1)) * sb.setWidth (2*(s+1))
+    let result : EFixedPoint (2*2^e + 2*(s+1)) (2^e + 2*s - 4) :=
+      {
+        state := .Number
+        num := {
+          sign := a.sign ^^ b.sign
+          val := prod.setWidth _ <<< shift
+          hExOffset := by omega
+        }
+      }
+    round _ _ m result
 
 theorem mul_comm (a b : PackedFloat 5 2) (m : RoundingMode)
-  : (mul (by omega) a b m) = (mul (by omega) b a m) := by
-  simp [mul, e_mul_comm]
+  : (mul a b m) = (mul b a m) := by
+  apply PackedFloat.inj
+  simp [mul, round, -BitVec.shiftLeft_eq', -BitVec.ushiftRight_eq']
+  bv_decide
+
+theorem mul_one_is_id (a : PackedFloat 5 2) (m : RoundingMode) (ha : ¬a.isNaN)
+  : (mul a Tests.oneE5M2 m) = a := by
+  apply PackedFloat.inj
+  simp at ha
+  simp [mul, round, BitVec.cons, Tests.oneE5M2, -BitVec.shiftLeft_eq', -BitVec.ushiftRight_eq']
+  bv_decide
