Fp/ExtraTheorems.lean
@@ -1,0 +1,14 @@
+import Fp.Basic
+import Fp.Addition
+import Fp.Multiplication
+import Fp.Rounding
+
+def twoE5M2 : PackedFloat 5 2 := PackedFloat.ofBits _ _ 0b01000000
+
+theorem add_eq_mul_two (a : PackedFloat 5 2) (m : RoundingMode)
+  : add (by omega) a a m = mul two a m := by
+  apply PackedFloat.inj
+  simp [add, e_add, f_add, twoE5M2, PackedFloat.toEFixed, mul, round,
+        BitVec.cons, -BitVec.shiftLeft_eq', -BitVec.ushiftRight_eq']
+  --bv_decide
+  sorry
